src/lib/state/DY.Lib.State.PrivateKeys.fst
@@ -68,6 +68,10 @@ let private_keys_pred #cinvs = {
   pred_knowable = (fun tr prin sess_id key value -> ());
 }
 
+val has_private_keys_functional_invariant: state_functional_predicate -> prop
+let has_private_keys_functional_invariant sfp =
+  has_map_functional_state_invariant #private_key_key #private_key_value sfp
+
 val has_private_keys_invariant: protocol_invariants -> prop
 let has_private_keys_invariant invs =
   has_map_session_invariant invs private_keys_pred
@@ -86,17 +90,29 @@ let private_key_type_to_usage sk_type =
 (*** Private Keys API ***)
 
 [@@ "opaque_to_smt"]
-val initialize_private_keys: prin:principal -> crypto nat
-let initialize_private_keys = initialize_map private_key_key private_key_value #_ // another workaround for FStarLang/FStar#3286
+val initialize_private_keys:
+  {|sfp:state_functional_predicate|} ->
+  #squash (has_private_keys_functional_invariant sfp) ->
+  prin:principal ->
+  crypto nat
+let initialize_private_keys #sfp #pf = initialize_map private_key_key private_key_value #_ #_ // another workaround for FStarLang/FStar#3286
 
 [@@ "opaque_to_smt"]
-val generate_private_key: principal -> nat -> private_key_type -> crypto (option unit)
+val generate_private_key:
+  {|sfp:state_functional_predicate|} ->
+  #squash (has_private_keys_functional_invariant sfp) ->
+  principal -> nat -> private_key_type ->
+  crypto (option unit)
 let generate_private_key prin sess_id sk_type =
   let* sk = mk_rand (private_key_type_to_usage sk_type) (principal_label prin) 64 in //TODO
   add_key_value prin sess_id ({ty = sk_type}) ({private_key = sk;})
 
 [@@ "opaque_to_smt"]
-val get_private_key: principal -> nat -> private_key_type -> crypto (option bytes)
+val get_private_key:
+  {|sfp:state_functional_predicate|} ->
+  #squash (has_private_keys_functional_invariant sfp) ->
+  principal -> nat -> private_key_type ->
+  crypto (option bytes)
 let get_private_key prin sess_id sk_type =
   let*? res = find_value prin sess_id ({ty = sk_type}) in
   return (Some res.private_key)
@@ -107,7 +123,8 @@ val initialize_private_keys_invariant:
   Lemma
   (requires
     trace_invariant tr /\
-    has_private_keys_invariant invs
+    has_private_keys_invariant invs /\
+    has_private_keys_functional_invariant invs.state_inv
   )
   (ensures (
     let (_, tr_out) = initialize_private_keys prin tr in
@@ -125,7 +142,8 @@ val generate_private_key_invariant:
   Lemma
   (requires
     trace_invariant tr /\
-    has_private_keys_invariant invs
+    has_private_keys_invariant invs /\
+    has_private_keys_functional_invariant invs.state_inv
   )
   (ensures (
     let (_, tr_out) = generate_private_key prin sess_id sk_type tr in
@@ -143,7 +161,8 @@ val get_private_key_invariant:
   Lemma
   (requires
     trace_invariant tr /\
-    has_private_keys_invariant invs
+    has_private_keys_invariant invs /\
+    has_private_keys_functional_invariant invs.state_inv
   )
   (ensures (
     let (opt_private_key, tr_out) = get_private_key prin sess_id pk_type tr in
